Making good progress.

src/svm.dfy
@@ -5,7 +5,7 @@ include "util.dfy"
  * memory, a sequence of bytecode instructions (and operands) and,
  * finally, a program counter.
  */
-type SVM = (stack<u16>,memory<u16>,seq<u8>,int)
+type SVM = (stack<u16>,memory<u16>,seq<u8>,u16)
 
 /**
  * Extract stack from machine state.
@@ -25,14 +25,20 @@ function code(vm:SVM) : seq<u8> { vm.2 }
 /**
  * Extract program counter from machine state.
  */
-function pc(vm:SVM) : int { vm.3 }
+function pc(vm:SVM) : u16 { vm.3 }
 
 /**
  * Machine is considered to be halted if the program counter 
  * is out-of-bounds.
  */
-function halted(vm:SVM) : bool { pc(vm) >= |code(vm)| }
+function halted(vm:SVM) : bool { pc(vm) >= (|code(vm)| as u16) }
 
+/**
+ * Force the machine into a halted state.
+ */
+function halt(vm:SVM) : SVM {
+		(vm.0,vm.1,vm.2,|vm.2| as u16)
+}
 /**
  * A valid Simple Virtual Machine requires a valid stack and a 
  * valid memory.  The program counter must also be valid with 
@@ -43,6 +49,75 @@ function validSVM(vm : SVM) : bool {
 }
 
 // =============================================================================
+// Simple Virtual Machine Opcodes
+// =============================================================================
+
+const NOP:u8 := 0x00;
+// Load constant onto stack
+const LDC:u8 := 0x01
+// Pop item off stack
+const POP:u8 := 0x02
+// Store top of stack to data
+const STORE:u8 := 0x03
+// Load data to stack
+const LOAD:u8 := 0x04
+// Add operands on stack
+const ADD:u8 := 0x05
+
+// =============================================================================
 // Instructions
 // =============================================================================
 
+// Execute a "single step" of the current program.
+function step(vm:SVM) : SVM
+// Virtual machine must be valid		
+requires validSVM(vm)
+// Virtual machine cannot be halted.
+requires !halted(vm) {
+				// decode
+				var opcode : u8 := svm_decode(vm);
+				//
+				var vm':SVM := svm_goto(vm, pc(vm)+1);
+				//
+				if opcode == NOP
+				then
+						stepNOP(vm')
+				else
+						// Opcodes requiring operand
+						var k : u8 := svm_decode(vm');
+						var vm'':SVM := svm_goto(vm', pc(vm')+1);
+						//
+						stepLDC(vm'',k)
+				// else
+				// 		halt(vm')
+}
+
+function stepNOP(vm:SVM) : SVM { vm }
+
+function stepLDC(vm:SVM, k:u8) : SVM {
+		if size(vm.0) < capacity(vm.0)
+		then
+				svm_push(vm,k)
+		else 
+				halt(vm)
+}
+
+// =============================================================================
+// Microcode
+// =============================================================================
+
+function svm_decode(vm:SVM) : u8 { vm.2[vm.3] }
+
+function svm_goto(vm:SVM, k:u16) : SVM { (vm.0,vm.1,vm.2,k) }
+
+function svm_push(vm:SVM, k:u8) : SVM {
+		(push(vm.0,k as u16),vm.1,vm.2,vm.3)
+}
+
+function svm_peek(vm:SVM) : u16 {
+		peek(vm.0)
+}
+
+function svm_pop(vm:SVM) : SVM {
+		(pop(vm.0),vm.1,vm.2,vm.3)
+}
